\begin{equation*}
        \begin{aligned}
            S' &= -\lambda S,\\
            E'_t &= q \lambda S - \epsilon E_t,\\
            I'_A &= p \epsilon E_{nt} + (1-c)p \epsilon E_t - r_a I_A,\\
            I'_S &= (1-d)(1-p) \epsilon E_{nt} + (1-c)(1-p) \epsilon E_t - r_s I_S,\\
            E'_{nt} &= (1-q) \lambda S - \epsilon E_{nt},\\
            I'_{Aq} &= c p \epsilon E_t - r_a I_{Aq},\\
            I'_{Sq} &= c(1-p) \epsilon E_t + d (1-p) \epsilon E_{nt} - r_s I_{Sq},\\
            H' &= \theta r_s (I_S + I_{Sq}) - \rho H,\\
            H'_{icu} &= \pi \rho H - \omega H_{icu},\\
            M' &= \mu \omega H_{icu} + \tau \rho H,\\
            R'_{obs} &= (1-\theta) r_s I_{Sq} + r_a I_{Aq} + (1-\pi-\tau)\rho H + (1-\mu)\omega H_{icu},\\
            R' &= (1-\theta) r_s I_S + r_a I_A.
        \end{aligned}
\end{equation*}